src/Init/Data/List/Range.lean
@@ -8,7 +8,7 @@ import Init.Data.List.Pairwise
 import Init.Data.List.Zip
 
 /-!
-# Lemmas about `List.range` and `List.enum`
+# Lemmas about `List.range` and `List.zipIdx`
 
 Most of the results are deferred to `Data.Init.List.Nat.Range`, where more results about
 natural arithmetic are available.
@@ -29,11 +29,15 @@ theorem range'_succ (s n step) : range' s (n + 1) step = s :: range' (s + step) 
   | 0 => rfl
   | _ + 1 => congrArg succ (length_range' _ _ _)
 
-@[simp] theorem range'_eq_nil : range' s n step = [] ↔ n = 0 := by
+@[simp] theorem range'_eq_nil_iff : range' s n step = [] ↔ n = 0 := by
   rw [← length_eq_zero, length_range']
 
-theorem range'_ne_nil (s : Nat) {n : Nat} : range' s n ≠ [] ↔ n ≠ 0 := by
+@[deprecated range'_eq_nil_iff (since := "2025-01-29")] abbrev range'_eq_nil := @range'_eq_nil_iff
+
+theorem range'_ne_nil_iff (s : Nat) {n step : Nat} : range' s n step ≠ [] ↔ n ≠ 0 := by
   cases n <;> simp
+
+@[deprecated range'_ne_nil_iff (since := "2025-01-29")] abbrev range'_ne_nil := @range'_ne_nil_iff
 
 @[simp] theorem range'_zero : range' s 0 step = [] := by
   simp
@@ -94,18 +98,18 @@ theorem range'_succ_left : range' (s + 1) n step = (range' s n step).map (· + 1
   · simp [Nat.add_right_comm]
 
 theorem range'_append : ∀ s m n step : Nat,
-    range' s m step ++ range' (s + step * m) n step = range' s (n + m) step
-  | _, 0, _, _ => rfl
+    range' s m step ++ range' (s + step * m) n step = range' s (m + n) step
+  | _, 0, _, _ => by simp
   | s, m + 1, n, step => by
     simpa [range', Nat.mul_succ, Nat.add_assoc, Nat.add_comm]
       using range'_append (s + step) m n step
 
 @[simp] theorem range'_append_1 (s m n : Nat) :
-    range' s m ++ range' (s + m) n = range' s (n + m) := by simpa using range'_append s m n 1
+    range' s m ++ range' (s + m) n = range' s (m + n) := by simpa using range'_append s m n 1
 
 theorem range'_sublist_right {s m n : Nat} : range' s m step <+ range' s n step ↔ m ≤ n :=
   ⟨fun h => by simpa only [length_range'] using h.length_le,
-   fun h => by rw [← Nat.sub_add_cancel h, ← range'_append]; apply sublist_append_left⟩
+   fun h => by rw [← add_sub_of_le h, ← range'_append]; apply sublist_append_left⟩
 
 theorem range'_subset_right {s m n : Nat} (step0 : 0 < step) :
     range' s m step ⊆ range' s n step ↔ m ≤ n := by
@@ -117,7 +121,7 @@ theorem range'_subset_right_1 {s m n : Nat} : range' s m ⊆ range' s n ↔ m �
   range'_subset_right (by decide)
 
 theorem range'_concat (s n : Nat) : range' s (n + 1) step = range' s n step ++ [s + step * n] := by
-  rw [Nat.add_comm n 1]; exact (range'_append s n 1 step).symm
+  exact (range'_append s n 1 step).symm
 
 theorem range'_1_concat (s n : Nat) : range' s (n + 1) = range' s n ++ [s + n] := by
   simp [range'_concat]
