src/Init/Data/Array/Lemmas.lean
@@ -3360,14 +3360,34 @@ theorem size_eq_length_toList (as : Array α) : as.size = as.toList.length := rf
 @[deprecated size_swapIfInBounds (since := "2024-11-24")] abbrev size_swap! := @size_swapIfInBounds
 
 @[simp] theorem size_range {n : Nat} : (range n).size = n := by
-  induction n <;> simp [range]
+  simp [range]
 
 @[simp] theorem toList_range (n : Nat) : (range n).toList = List.range n := by
   apply List.ext_getElem <;> simp [range]
 
 @[simp]
-theorem getElem_range {n : Nat} {x : Nat} (h : x < (Array.range n).size) : (Array.range n)[x] = x := by
+theorem getElem_range {n : Nat} {i : Nat} (h : i < (Array.range n).size) : (Array.range n)[i] = i := by
   simp [← getElem_toList]
+
+theorem getElem?_range {n : Nat} {i : Nat} : (Array.range n)[i]? = if i < n then some i else none := by
+  simp [getElem?_def, getElem_range]
+
+@[simp] theorem size_range' {start size step} : (range' start size step).size = size := by
+  simp [range']
+
+@[simp] theorem toList_range' {start size step} :
+     (range' start size step).toList = List.range' start size step := by
+  apply List.ext_getElem <;> simp [range']
+
+@[simp]
+theorem getElem_range' {start size step : Nat} {i : Nat}
+    (h : i < (Array.range' start size step).size) :
+    (Array.range' start size step)[i] = start + step * i := by
+  simp [← getElem_toList]
+
+theorem getElem?_range' {start size step : Nat} {i : Nat} :
+    (Array.range' start size step)[i]? = if i < size then some (start + step * i) else none := by
+  simp [getElem?_def, getElem_range']
 
 /-! ### shrink -/
 
@@ -3646,6 +3666,11 @@ theorem uset_toArray (l : List α) (i : USize) (a : α) (h : i.toNat < l.toArray
   simp [Function.comp_def]
 
 @[simp] theorem toArray_range (n : Nat) : (range n).toArray = Array.range n := by
+  apply ext'
+  simp
+
+@[simp] theorem toArray_range' (start size step : Nat) :
+    (range' start size step).toArray = Array.range' start size step := by
   apply ext'
   simp
 
